candle/standard/opentheory/readerProgScript.sml
@@ -52,7 +52,7 @@ val _ = (append_prog o process_topdecs) ‘
 Definition l2c_aux_sem_def:
   (l2c_aux_sem acc [] = REVERSE acc) ∧
   (l2c_aux_sem acc (h::t) =
-    l2c_aux_sem (tokenize (implode (str_prefix h))::acc) t)
+    l2c_aux_sem (tokenize (str_prefix (implode h))::acc) t)
 End
 
 Theorem l2c_aux_sem_MAP:
@@ -63,6 +63,9 @@ Proof
   Induct_on ‘ls’
   \\ rw [l2c_aux_sem_def]
 QED
+
+Theorem reverse_spec[local] =
+  INST_TYPE [alpha |-> “:command”] ListProgTheory.reverse_v_thm;
 
 Theorem l2c_aux_spec:
   ∀n fs fd fdv ls lsv.
@@ -78,42 +81,38 @@ Theorem l2c_aux_spec:
           STDIO (fastForwardFD fs fd))
 Proof
   Induct_on ‘linesFD fs fd’
-  >-
-   (rpt strip_tac
-    \\ qpat_x_assum ‘[] = _’ (assume_tac o SYM)
-    \\ xcf "l2c_aux" (get_ml_prog_state ())
-    \\ ‘IS_SOME (get_file_content fs fd)’
+  \\ rpt strip_tac
+  \\ xcf "l2c_aux" (get_ml_prog_state ())
+  \\ qpat_x_assum ‘_ = linesFD fs fd’ (assume_tac o SYM) \\ fs []
+  \\ ‘IS_SOME (get_file_content fs fd)’
       by fs []
+  >-
+   (xlet_auto >- xsimpl
     \\ ‘lineFD fs fd = NONE’
       by fs [linesFD_nil_lineFD_NONE]
-    \\ xlet_auto
-    >- xsimpl
     \\ fs [OPTION_TYPE_def, l2c_aux_sem_def]
     \\ xmatch
-    \\ xapp_spec (INST_TYPE [alpha |-> “:command”]
-                            ListProgTheory.reverse_v_thm)
+    \\ xapp_spec reverse_spec
     \\ instantiate
     \\ simp [lineFD_NONE_lineForwardFD_fastForwardFD]
     \\ xsimpl)
-  \\ rpt strip_tac
-  \\ xcf "l2c_aux" (get_ml_prog_state ())
-  \\ qpat_x_assum ‘_::_ = _’ (assume_tac o SYM)
   \\ drule linesFD_cons_imp
   \\ strip_tac \\ rveq \\ fs []
   \\ xlet_auto >- xsimpl
   \\ fs [OPTION_TYPE_def, l2c_aux_sem_MAP]
   \\ xmatch
   \\ xlet_auto >- xsimpl
+  \\ xlet_auto >- xsimpl
   \\ xlet_auto >- (xcon \\ xsimpl)
   \\ xapp
-  \\ qexists_tac ‘emp’
-  \\ xsimpl
+  \\ CONV_TAC SWAP_EXISTS_CONV
   \\ Q.REFINE_EXISTS_TAC ‘x::xs’
-  \\ simp [LIST_TYPE_def]
+  \\ simp [LIST_TYPE_def, o_DEF]
   \\ goal_assum (first_assum o mp_then Any mp_tac) \\ fs []
   \\ goal_assum (first_assum o mp_then Any mp_tac) \\ fs []
-  \\ Q.LIST_EXISTS_TAC [‘lineForwardFD fs fd’, ‘fd’] \\ simp []
-  \\ drule get_file_content_lineForwardFD_forwardFD \\ rw []
+  \\ Q.LIST_EXISTS_TAC [‘emp’, ‘lineForwardFD fs fd’, ‘fd’]
+  \\ drule get_file_content_lineForwardFD_forwardFD
+  \\ strip_tac \\ fs []
   \\ xsimpl
   \\ metis_tac [APPEND_ASSOC, CONS_APPEND]
 QED
@@ -181,9 +180,7 @@ Proof
   \\ ‘CARD (set (MAP FST fs.infds)) < fs.maxFD’
     by fs []
   \\ reverse (Cases_on ‘STD_streams fs’)
-  >-
-   (fs [STDIO_def]
-    \\ xpull)
+  >- (fs [STDIO_def] \\ xpull)
   \\ reverse (Cases_on ‘consistentFS fs’)
   >-
    (fs [STDIO_def, IOFS_def, wfFS_def]
@@ -208,16 +205,15 @@ Proof
   \\ imp_res_tac nextFD_ltX
   \\ progress inFS_fname_ALOOKUP_EXISTS
   \\ progress ALOOKUP_inFS_fname_openFileFS_nextFD
-  \\ rfs[]
+  \\ rfs []
   \\ pop_assum (qspec_then ‘0’ strip_assume_tac)
   \\ qmatch_assum_abbrev_tac ‘validFD fd fso’
   \\ imp_res_tac inFS_fname_ALOOKUP_EXISTS
   \\ ‘∃c. get_file_content fso fd = SOME (c, 0)’
     by fs [get_file_content_def, validFD_def, Abbr ‘fso’, openFileFS_inode_tbl]
   \\ ‘get_mode fso fd = SOME ReadMode’
-  by fs [Abbr ‘fso’, openFileFS_def, get_mode_def, get_file_content_fsupdate]
-  \\ xlet_auto
-  >- xsimpl
+    by fs [Abbr ‘fso’, openFileFS_def, get_mode_def, get_file_content_fsupdate]
+  \\ xlet_auto >- xsimpl
   \\ xlet_auto_spec (SOME closeIn_STDIO_spec)
   >-
    (xsimpl
@@ -232,8 +228,8 @@ Proof
     \\ rfs[]
     \\ fsrw_tac [SATISFY_ss] [Abbr ‘fso’])
   \\ xcon
-  \\ simp [OPTION_TYPE_def]
-  \\ fs [get_file_content_def, Abbr ‘fso’, openFileFS_inode_tbl]
+  \\ fs [OPTION_TYPE_def, get_file_content_def, Abbr ‘fso’,
+         openFileFS_inode_tbl]
   \\ imp_res_tac linesFD_openFileFS_nextFD \\ rfs []
   \\ first_x_assum (qspec_then ‘ReadMode’ mp_tac) \\ strip_tac \\ fs []
   \\ fs [MAP_MAP_o]
@@ -252,6 +248,7 @@ QED
 
 (*
  * Read all input from stdin.
+ * Uses the regular (unbuffered) I/O.
  *)
 
 val _ = (append_prog o process_topdecs) `
@@ -289,7 +286,7 @@ val _ = (append_prog o process_topdecs) `
  *)
 
 val _ = (append_prog o process_topdecs) `
-  fun read_file_buffered file =
+  fun read_file file =
     case TextIO.b_inputAllTokensFrom file is_newline tokenize of
       None =>
         TextIO.output TextIO.stdErr (msg_bad_name file)
@@ -301,6 +298,18 @@ val _ = (append_prog o process_topdecs) `
         end
         handle Kernel.Fail e => TextIO.output TextIO.stdErr e;
   `;
+
+Theorem POSTve_POSTv[local]:
+  ∀Q. POSTve Q (λx. SEP_F) = $POSTv Q
+Proof
+  rw [SEP_CLAUSES, POSTv_def, POSTve_def]
+QED
+
+Theorem context_spec =
+  context_spec
+  |> Q.SPEC ‘()’
+  |> SIMP_RULE (srw_ss())
+    [context_def, get_the_context_def, SEP_CLAUSES, POSTve_POSTv];
 
 Theorem read_stdin_spec:
   UNIT_TYPE () uv ∧
@@ -314,86 +323,56 @@ Theorem read_stdin_spec:
 Proof
   xcf "read_stdin" (get_ml_prog_state ())
   \\ reverse (Cases_on `STD_streams fs`)
-  >- (fs [TextIOProofTheory.STDIO_def] \\ xpull)
-  \\ fs [UNIT_TYPE_def]
-  \\ simp [read_stdin_def]
+  >- (fs [STDIO_def] \\ xpull)
+  \\ fs [UNIT_TYPE_def, read_stdin_def]
   \\ assume_tac INSTREAM_stdin
   \\ drule stdin_get_file_content \\ strip_tac
   \\ drule STD_streams_get_mode \\ strip_tac
   \\ assume_tac init_state_v_thm
+  \\ drule linesFD_splitlines_get_stdin
+  \\ disch_then (assume_tac o SYM)
+  \\ drule stdin_get_stdin \\ strip_tac \\ fs []
   \\ xmatch
   \\ CASE_TAC \\ fs []
-  \\ CASE_TAC \\ fs []
+  \\ CASE_TAC \\ CASE_TAC \\ fs []
   >-
-   (CASE_TAC \\ fs []
-    \\ qmatch_goalsub_abbrev_tac ‘$POSTv Q’
+   (
+    qmatch_goalsub_abbrev_tac ‘$POSTv Q’
     \\ xhandle ‘$POSTv Q’ \\ xsimpl
     \\ xlet_auto >- xsimpl
-    \\ xlet_auto
-    >- xsimpl
+    \\ xlet_auto \\ xsimpl
     >-
-     (xsimpl
-      \\ rpt gen_tac
-      \\ strip_tac
-      \\ drule linesFD_splitlines_get_stdin
-      \\ disch_then (assume_tac o SYM)
-      \\ drule stdin_get_stdin \\ strip_tac \\ fs []
-      \\ fs [lines_of_def, MAP_MAP_o, stdin_def, o_DEF]
-      \\ rfs []
-      \\ fs [strcat_thm])
+     (rpt gen_tac \\ strip_tac
+      \\ fs [lines_of_def, MAP_MAP_o, stdin_def, o_DEF, strcat_thm]
+      \\ rfs [])
     \\ xlet_auto >- xsimpl
     \\ xlet_auto >- (xcon \\ xsimpl)
-    \\ rename1 ‘(Success st1p, refs1)’
-    \\ drule context_spec
-    \\ disch_then (qspecl_then [‘p’, ‘refs1’] mp_tac)
-    \\ simp [context_def, get_the_context_def, SEP_CLAUSES]
-    \\ ‘∀Q. POSTve Q (λx. SEP_F) = $POSTv Q’
-      by rw [POSTve_def, POSTv_def, SEP_CLAUSES]
-    \\ simp []
-    \\ strip_tac
+    \\ rename1 ‘(Success _, refs1)’
+    \\ drule_then (qspecl_then [‘p’, ‘refs1’] strip_assume_tac) context_spec
     \\ xlet_auto >- xsimpl
     \\ xlet_auto >- xsimpl
     \\ xapp
     \\ qunabbrev_tac ‘Q’
     \\ instantiate
     \\ xsimpl
-    \\ drule linesFD_splitlines_get_stdin
-    \\ disch_then (assume_tac o SYM)
-    \\ drule stdin_get_stdin \\ strip_tac \\ fs []
-    \\ fs [lines_of_def, MAP_MAP_o, stdin_def, o_DEF]
+    \\ fs [lines_of_def, MAP_MAP_o, stdin_def, o_DEF, strcat_thm]
     \\ rfs []
-    \\ fs [strcat_thm]
     \\ rveq \\ fs []
     \\ Q.LIST_EXISTS_TAC [‘HOL_STORE r’, ‘fastForwardFD fs 0’]
     \\ simp [add_stdout_fastForwardFD]
     \\ xsimpl
     \\ rw [UNIT_TYPE_def])
-  \\ CASE_TAC \\ fs []
   \\ xhandle ‘POSTe ev.
                 &HOL_EXN_TYPE (Fail m) ev *
                 HOL_STORE r *
                 STDIO (fastForwardFD fs 0)’
   >-
    (xlet_auto >- xsimpl
-    \\ xlet_auto
-    >- xsimpl
-    >-
-     (xsimpl
-      \\ rpt gen_tac
-      \\ strip_tac
-      \\ drule linesFD_splitlines_get_stdin
-      \\ disch_then (assume_tac o SYM)
-      \\ drule stdin_get_stdin \\ strip_tac \\ fs []
-      \\ fs [lines_of_def, MAP_MAP_o, stdin_def, o_DEF]
-      \\ rfs []
-      \\ fs [strcat_thm]
-      \\ xsimpl)
-    \\ drule linesFD_splitlines_get_stdin
-    \\ disch_then (assume_tac o SYM)
-    \\ drule stdin_get_stdin \\ strip_tac \\ fs []
-    \\ fs [lines_of_def, MAP_MAP_o, stdin_def, o_DEF]
+    \\ xlet_auto \\ xsimpl
+    \\ rpt gen_tac \\ rpt strip_tac
+    \\ fs [lines_of_def, MAP_MAP_o, stdin_def, o_DEF, strcat_thm]
     \\ rfs []
-    \\ fs [strcat_thm])
+    \\ xsimpl)
   \\ fs [HOL_EXN_TYPE_def]
   \\ xcases
   \\ xapp_spec output_stderr_spec
@@ -401,6 +380,26 @@ Proof
   \\ Q.LIST_EXISTS_TAC [‘HOL_STORE r’, ‘fastForwardFD fs 0’]
   \\ xsimpl
   \\ rw [UNIT_TYPE_def]
+QED
+
+Theorem b_inputAllTokensFrom_spec2:
+  FILENAME fn fnv ∧
+  hasFreeFD fs ⇒
+    app (p: 'ffi ffi_proj) TextIO_b_inputAllTokensFrom_v
+      [fnv; is_newline_v; tokenize_v]
+      (STDIO fs)
+      (POSTv sv.
+        &OPTION_TYPE (LIST_TYPE (LIST_TYPE READER_COMMAND_TYPE))
+          (if inFS_fname fs fn then
+            SOME (MAP (MAP tokenize ∘ tokens is_newline)
+                      (all_lines fs fn))
+           else
+             NONE) sv *
+        STDIO fs)
+Proof
+  strip_tac
+  \\ irule b_inputAllTokensFrom_spec
+  \\ simp [theorem "is_newline_v_thm", tokenize_v_thm, is_newline_def]
 QED
 
 Theorem read_file_spec:
@@ -418,93 +417,7 @@ Proof
   >- (fs [TextIOProofTheory.STDIO_def] \\ xpull)
   \\ reverse (Cases_on`consistentFS fs`)
   >- (fs [STDIO_def,IOFS_def,wfFS_def,consistentFS_def] \\ xpull \\ metis_tac[])
-  \\ xlet_auto >- xsimpl
-  \\ simp[read_file_def]
-  \\ reverse IF_CASES_TAC \\ fs [OPTION_TYPE_def]
-  >-
-   (xmatch
-    \\ xlet_auto >- xsimpl
-    \\ xapp_spec output_stderr_spec
-    \\ instantiate
-    \\ Q.LIST_EXISTS_TAC [‘HOL_STORE refs’, ‘fs’]
-    \\ xsimpl)
-  \\ xmatch
-  \\ CASE_TAC \\ fs []
-  \\ CASE_TAC \\ fs []
-  >-
-   (CASE_TAC \\ fs []
-    \\ qmatch_goalsub_abbrev_tac ‘$POSTv Q’
-    \\ xhandle ‘$POSTv Q’ \\ xsimpl
-    \\ qunabbrev_tac ‘Q’
-    \\ assume_tac init_state_v_thm
-    \\ xlet_auto
-    >- xsimpl
-    >- xsimpl
-    \\ xlet_auto >- xsimpl
-    \\ xlet_auto >- (xcon \\ xsimpl)
-    \\ rename1 ‘(Success (st1,_), refs1)’
-    \\ drule context_spec
-    \\ disch_then (qspecl_then [‘p’, ‘refs1’] mp_tac)
-    \\ simp [context_def, get_the_context_def, SEP_CLAUSES]
-    \\ ‘∀Q. POSTve Q (λx. SEP_F) = $POSTv Q’
-      by rw [POSTve_def, POSTv_def, SEP_CLAUSES]
-    \\ simp []
-    \\ strip_tac
-    \\ xlet_auto >- xsimpl
-    \\ xlet_auto >- xsimpl
-    \\ xapp
-    \\ instantiate
-    \\ rveq \\ fs []
-    \\ Q.LIST_EXISTS_TAC [‘HOL_STORE refs'’, ‘fs’]
-    \\ xsimpl)
-  \\ CASE_TAC \\ fs []
-  \\ xhandle ‘POSTe ev.
-                &HOL_EXN_TYPE (Fail m) ev *
-                HOL_STORE r *
-                STDIO fs’
-  >-
-   (assume_tac init_state_v_thm
-    \\ xlet_auto \\ xsimpl)
-  \\ fs [HOL_EXN_TYPE_def]
-  \\ xcases
-  \\ xapp_spec output_stderr_spec
-  \\ instantiate
-  \\ Q.LIST_EXISTS_TAC [‘HOL_STORE r’, ‘fs’]
-  \\ xsimpl
-QED
-
-
-Theorem b_inputAllTokensFrom_spec2 =
-  GEN_ALL b_inputAllTokensFrom_spec |>
-  Q.ISPECL [
-    ‘p: 'ffi ffi_proj’,
-    ‘tokenize_v’,
-    ‘tokenize’,
-    ‘is_newline_v’,
-    ‘fs: IO_fs’,
-    ‘fnamev: v’,
-    ‘fname: mlstring’,
-    ‘is_newline’,
-    ‘READER_COMMAND_TYPE’
-  ] |>
-  SIMP_RULE bool_ss
-    [theorem "is_newline_v_thm", tokenize_v_thm, is_newline_def];
-
-Theorem read_file_buffered_spec:
-  FILENAME fnm fnv ∧
-  hasFreeFD fs ⇒
-    app (p: 'ffi ffi_proj) read_file_buffered_v [fnv]
-      (STDIO fs * HOL_STORE refs)
-      (POSTv u.
-        &UNIT_TYPE () u *
-        STDIO (FST (read_file_buffered fs refs fnm)) *
-        HOL_STORE (FST (SND (read_file_buffered fs refs fnm))))
-Proof
-  xcf "read_file_buffered" (get_ml_prog_state())
-  \\ reverse (Cases_on `STD_streams fs`)
-  >- (fs [TextIOProofTheory.STDIO_def] \\ xpull)
-  \\ reverse (Cases_on`consistentFS fs`)
-  >- (fs [STDIO_def,IOFS_def,wfFS_def,consistentFS_def] \\ xpull \\ metis_tac[])
+  \\ assume_tac init_state_v_thm
   \\ xlet ‘POSTv sv.
              &OPTION_TYPE (LIST_TYPE (LIST_TYPE READER_COMMAND_TYPE))
                (if inFS_fname fs fnm then
@@ -518,7 +431,7 @@ Proof
    (xapp_spec b_inputAllTokensFrom_spec2
     \\ instantiate
     \\ xsimpl)
-  \\ simp [read_file_buffered_def]
+  \\ simp [read_file_def]
   \\ reverse IF_CASES_TAC \\ fs [OPTION_TYPE_def]
   >-
    (xmatch
@@ -535,24 +448,15 @@ Proof
     \\ xhandle ‘$POSTv Q’ \\ xsimpl
     \\ qunabbrev_tac ‘Q’
     \\ xlet_auto >- xsimpl
-    \\ assume_tac init_state_v_thm
-    \\ xlet_auto
-    >- xsimpl
-    >- xsimpl
+    \\ xlet_auto \\ xsimpl
     \\ xlet_auto >- xsimpl
     \\ xlet_auto >- (xcon \\ xsimpl)
     \\ rveq \\ fs []
     \\ rename1 ‘(Success _, refs1)’
-    \\ drule context_spec
-    \\ disch_then (qspecl_then [‘p’, ‘refs1’] mp_tac)
-    \\ simp [context_def, get_the_context_def, SEP_CLAUSES]
-    \\ ‘∀Q. POSTve Q (λx. SEP_F) = $POSTv Q’
-      by rw [POSTve_def, POSTv_def, SEP_CLAUSES]
-    \\ simp []
-    \\ strip_tac
+    \\ drule_then (qspecl_then [‘p’, ‘refs1’] strip_assume_tac) context_spec
+    \\ xlet_auto >- xsimpl
     \\ xlet_auto >- xsimpl
     \\ rveq \\ fs []
-    \\ xlet_auto >- xsimpl
     \\ xapp
     \\ instantiate
     \\ Q.LIST_EXISTS_TAC [‘HOL_STORE refs'’, ‘fs’]
@@ -562,8 +466,7 @@ Proof
                 HOL_STORE r *
                 STDIO fs’
   >-
-   (xlet_auto >- xsimpl
-    \\ assume_tac init_state_v_thm
+   (xlet_auto \\ xsimpl
     \\ xlet_auto \\ xsimpl)
   \\ fs [HOL_EXN_TYPE_def]
   \\ xcases
@@ -573,11 +476,6 @@ Proof
   \\ xsimpl
 QED
 
-(* TODO
- * - Tidy up! All of these theorems are basically the same copy-paste
- *   over and over.
- *)
-
 val _ = (append_prog o process_topdecs) `
   fun reader_main u =
     let
@@ -585,15 +483,28 @@ val _ = (append_prog o process_topdecs) `
     in
       case CommandLine.arguments () of
         [] => read_stdin ()
-      | ["--nobuf", file] => read_file file
-      | [file] => read_file_buffered file
+      | [file] => read_file file
       | _ => TextIO.output TextIO.stdErr msg_usage
       end
   `;
 
-(* TODO:
- * Awful everything, fix
- *)
+Theorem init_reader_spec:
+  ∀uv state.
+    (∃s. init_reader () refs = (Success (), s)) ∧
+    UNIT_TYPE () uv ⇒
+      app (p: 'ffi ffi_proj) init_reader_v [uv]
+        (HOL_STORE refs)
+        (POSTv rv.
+          SEP_EXISTS refs'.
+            HOL_STORE refs' *
+            &(init_reader () refs = (Success (),refs')) *
+            &UNIT_TYPE () rv)
+Proof
+  rw []
+  \\ drule_then (qspecl_then [‘p’, ‘refs’] assume_tac) init_reader_spec
+  \\ rfs [POSTve_POSTv, SEP_CLAUSES]
+QED
+
 Theorem reader_main_spec:
   (∃s. init_reader () refs = (Success (), s)) ∧
   input_exists fs cl ⇒
@@ -604,8 +515,52 @@ Theorem reader_main_spec:
         &UNIT_TYPE () u *
         STDIO (FST (reader_main fs refs (TL cl))))
 Proof
-  cheat (* Probably true but way too annoying with the pattern match *)
-        (* on the string literal ... *)
+  xcf "reader_main" (get_ml_prog_state ())
+  \\ reverse (Cases_on ‘wfcl cl’)
+  >- (simp [COMMANDLINE_def] \\ xpull)
+  \\ xlet_auto >- (xcon \\ xsimpl)
+  \\ xlet_auto >- xsimpl
+  \\ xlet_auto >- (xcon \\ xsimpl)
+  \\ xlet_auto_spec (SOME CommandLine_arguments_spec)
+  >- xsimpl
+  \\ fs [input_exists_def]
+  \\ simp [reader_main_def]
+  \\ CASE_TAC \\ fs []
+  >-
+   (fs [LIST_TYPE_def]
+    \\ xmatch
+    \\ xlet_auto >- (xcon \\ xsimpl)
+    \\ xapp
+    \\ simp [PULL_EXISTS]
+    \\ goal_assum (first_assum o mp_then Any mp_tac) \\ fs []
+    \\ Q.LIST_EXISTS_TAC [‘COMMANDLINE cl’, ‘refs'’]
+    \\ xsimpl)
+  \\ Cases_on `t` \\ fs [LIST_TYPE_def]
+  >-
+   (Cases_on ‘h’ \\ fs [STRING_TYPE_def] \\ rveq
+    \\ Cases_on ‘cl’ \\ fs [] \\ rveq
+    \\ xmatch
+    \\ IF_CASES_TAC >- (pop_assum mp_tac \\ EVAL_TAC)
+    \\ reverse conj_tac >- (EVAL_TAC \\ fs [])
+    \\ xapp
+    \\ simp [PULL_EXISTS]
+    \\ goal_assum (first_assum o mp_then Any mp_tac) \\ fs []
+    \\ rename1 ‘StrLit ss’
+    \\ qmatch_goalsub_abbrev_tac ‘COMMANDLINE cl’
+    \\ Q.LIST_EXISTS_TAC [‘COMMANDLINE cl’, ‘refs'’, ‘strlit ss’]
+    \\ fs [FILENAME_def, wfcl_def, validArg_def, Abbr ‘cl’]
+    \\ xsimpl)
+  \\ rveq \\ fs []
+  \\ rename1 ‘TL cl = x1::x2::x3’
+  \\ Cases_on `x1` \\ Cases_on `x2` \\ fs [STRING_TYPE_def]
+  \\ xmatch
+  \\ IF_CASES_TAC >- (pop_assum mp_tac \\ EVAL_TAC)
+  \\ reverse conj_tac >- (EVAL_TAC \\ fs [])
+  \\ reverse conj_tac >- (EVAL_TAC \\ fs [])
+  \\ xapp_spec output_stderr_spec
+  \\ Q.LIST_EXISTS_TAC [‘COMMANDLINE cl * HOL_STORE refs'’, ‘msg_usage’, ‘fs’]
+  \\ xsimpl
+  \\ simp [msg_usage_v_thm]
 QED
 
 (* ------------------------------------------------------------------------- *)
@@ -613,27 +568,20 @@ QED
 (* ------------------------------------------------------------------------- *)
 
 Theorem reader_whole_prog_spec:
-   input_exists fs cl ⇒
-     whole_prog_spec reader_main_v cl fs (SOME (HOL_STORE init_refs))
-       ((=) (FST (reader_main fs init_refs (TL cl))))
+  input_exists fs cl ⇒
+    whole_prog_spec reader_main_v cl fs (SOME (HOL_STORE init_refs))
+      ((=) (FST (reader_main fs init_refs (TL cl))))
 Proof
   rw [whole_prog_spec_def]
-  \\ qmatch_goalsub_abbrev_tac `fs1 = _ with numchars := _`
-  \\ qexists_tac `fs1` \\ fs [Abbr`fs1`]
+  \\ qmatch_goalsub_abbrev_tac ‘fs1 = _ with numchars := _’
+  \\ qexists_tac ‘fs1’ \\ qunabbrev_tac ‘fs1’
   \\ reverse conj_tac
-  >- cheat (* TODO this theorem too becomes annoying *) (*
-   (fs [reader_main_def, read_file_def, read_stdin_def, read_file_buffered_def]
+  >-
+   (fs [reader_main_def, read_stdin_def, read_file_def]
     \\ rpt (PURE_CASE_TAC \\ fs [])
     \\ fs [GSYM add_stdo_with_numchars, with_same_numchars]
-    \\ metis_tac [fastForwardFD_with_numchars, with_same_numchars]) *)
-  \\ irule (reader_main_spec
-            |> UNDISCH |> MATCH_MP app_wgframe
-            |> MP_CANON |> DISCH_ALL
-            |> SIMP_RULE (srw_ss()) [])
-  \\ xsimpl \\ instantiate
-  \\ xsimpl
-  \\ CONV_TAC SWAP_EXISTS_CONV
-  \\ qexists_tac `init_refs` \\ xsimpl
+    \\ metis_tac [fastForwardFD_with_numchars, with_same_numchars])
+  \\ irule reader_main_spec
   \\ Cases_on `init_reader () init_refs`
   \\ drule init_reader_success \\ rw []
 QED
